Add op for float max and min for x86.
The ops `Omaxf` and `Ominf` have the same semantics as `minsd` and
`maxsd` instruction, i.e. if both arguments are equal the second
argument is returned as well as for NaN.

The operations are the used in SelectOp to implement the built-in
function `__builtin_fmax` and `__builtin_fmin`.
Bug 32640

x86/Asmexpand.ml
@@ -408,24 +408,6 @@ let expand_builtin_inline name args res =
   (* Float arithmetic *)
   | ("__builtin_fsqrt" | "__builtin_sqrt"), [BA(FR a1)], BR(FR res) ->
      emit (Psqrtsd (res,a1))
-  | "__builtin_fmax", [BA(FR a1); BA(FR a2)], BR(FR res) ->
-     if res = a1 then
-       emit (Pmaxsd (res,a2))
-     else if res = a2 then
-       emit (Pmaxsd (res,a1))
-     else begin
-	 emit (Pmovsd_ff (res,a1));
-	 emit (Pmaxsd (res,a2))
-       end
-  | "__builtin_fmin", [BA(FR a1); BA(FR a2)], BR(FR res) ->
-     if res = a1 then
-       emit (Pminsd (res,a2))
-     else if res = a2 then
-       emit (Pminsd (res,a1))
-     else begin
-	 emit (Pmovsd_ff (res,a1));
-	 emit (Pminsd (res,a2))
-       end
   | "__builtin_fmadd",  _, _ ->
       expand_fma args res
         (fun r1 r2 r3 -> Pfmadd132(r1, r2, r3))
